first seminar content

Sem I/sem1.dfy
@@ -1,3 +1,100 @@
-method Main() {
-  print "Hello, World!\n";
+predicate isNatural(x: int)
+{
+    x >= 0
 }
+
+lemma L1()
+    ensures isNatural(8);
+    {
+        //
+    }
+
+newtype natural = x: int | isNatural(x)
+
+lemma NatSum(x: int, y: int)
+    ensures isNatural(x) && isNatural(y) ==> isNatural(x+y)
+    {
+        //
+    }
+
+function min32(): int
+{
+    -214783648
+}
+
+function max32(): int
+{
+    214783647
+}
+
+predicate isInt32(x: int)
+{
+    min32() <= x <= max32()
+}
+
+newtype int32 = x: int | isInt32(x)
+
+function add32(x: int32, y:int32) : int32
+{
+    var res := x as int + y as int;
+
+    if (isInt32(res)) then res as int32
+    else if (res < min32()) then (max32() + 1 - min32() + res) as int32
+    else (res - max32()) as int32
+}
+
+lemma MinusInt32(x: int)
+requires isInt32(x)
+ensures x > min32() ==> isInt32(-x)
+{
+    //
+}
+
+function minus32(x: int32) : int32
+{
+    if(x == min32() as int32) then x else -x
+}
+
+lemma Minus()
+ensures forall x: int32 :: add32(x, minus32(x)) == 0 as int32
+{
+    //
+}
+
+lemma CommAdd32(x: int32, y: int32)
+    ensures add32(x, y) == add32(y, x)
+    {
+        //
+    }
+
+predicate IsPrime(x: natural)
+{
+    x >= 2 && forall y: natural :: 2 <= y < x ==> x % y != 0
+}
+
+// lemma InfinitePrimeNumbers()
+// ensures forall x: natural :: exists y: natural :: IsPrime(y) && y > x 
+// {
+//     //
+// }
+
+lemma TwoIsPrime(x: natural)
+requires IsPrime(x) && x > 2
+ensures x % 2 != 0
+{
+    //
+}
+
+lemma EveryPrimeNumberNotTwoIsOdd(x: natural)
+requires IsPrime(x) && x > 2
+ensures !IsPrime(x + 1)
+{
+    TwoIsPrime(x);
+    assert (x + 1) % 2 == 0;
+}
+
+predicate SixK1(x: natural) 
+{
+    IsPrime(x) && x >= 5 ==> exists k: int :: x as int == 6*k + 1 || x as int == 6*k + 5
+}
+
